theories/Logic/PA_cyclic.v
@@ -98,22 +98,22 @@ Inductive PA_cyclic_pre : formula -> nat -> ord -> list formula -> Type :=
 | oneloop1 : forall {A : formula} {n : nat} {d1 d2 : nat} {alpha1 alpha2 : ord} (L1 L2 : list formula) (LSTC : free_list A = [n] \/ free_list A = []),
     PA_cyclic_pre (substitution A n zero) d1 alpha1 L1 ->
     PA_cyclic_pre (substitution A n (succ (var n))) d2 alpha2 L2 ->
-    PA_cyclic_pre (univ n A) (max d1 d2) (ord_succ (ord_add (ord_mult alpha2 (wcon (wcon Zero 0 Zero) 0 Zero)) alpha1)) ((remove form_eq_dec A L2) ++ L1)
+    PA_cyclic_pre (univ n A) (max d1 d2) (ord_succ (ord_add alpha1 (ord_mult alpha2 (wcon (wcon Zero 0 Zero) 0 Zero)))) ((remove form_eq_dec A L2) ++ L1)
 
 | oneloop2 : forall {C A : formula} {n : nat} {d1 d2 : nat} {alpha1 alpha2 : ord} (L1 L2 : list formula) (LSTC : free_list A = [n] \/ free_list A = []) (CC : closed C = true),
     PA_cyclic_pre (lor C (substitution A n zero)) d1 alpha1 L1 ->
     PA_cyclic_pre (substitution A n (succ (var n))) d2 alpha2 L2 ->
-    PA_cyclic_pre (lor C (univ n A)) (max d1 d2) (ord_succ (ord_add (ord_mult alpha2 (wcon (wcon Zero 0 Zero) 0 Zero)) alpha1)) ((remove form_eq_dec A L2) ++ L1)
+    PA_cyclic_pre (lor C (univ n A)) (max d1 d2) (ord_succ (ord_add alpha1 (ord_mult alpha2 (wcon (wcon Zero 0 Zero) 0 Zero)))) ((remove form_eq_dec A L2) ++ L1)
 
 | multloop1 : forall {A : formula} {n : nat} {d1 d2 : nat} {alpha1 alpha2 : ord} (L1 L2 : list formula) (LSTN : free_list A <> [n] /\ free_list A <> []),
     PA_cyclic_pre (substitution A n zero) d1 alpha1 L1 ->
     PA_cyclic_pre (substitution A n (succ (var n))) d2 alpha2 L2 ->
-    PA_cyclic_pre (univ n A) (max d1 d2) (ord_succ (ord_add (ord_mult alpha2 (wcon (wcon Zero 0 Zero) 0 Zero)) alpha1)) (((univ n A) :: remove form_eq_dec A L2) ++ L1)
+    PA_cyclic_pre (univ n A) (max d1 d2) (ord_succ (ord_add alpha1 (ord_mult alpha2 (wcon (wcon Zero 0 Zero) 0 Zero)))) (((univ n A) :: remove form_eq_dec A L2) ++ L1)
 
 | multloop2 : forall {C A : formula} {n : nat} {d1 d2 : nat} {alpha1 alpha2 : ord} (L1 L2 : list formula) (LSTN : (free_list A <> [n] /\ free_list A <> []) \/ closed C = false),
     PA_cyclic_pre (lor C (substitution A n zero)) d1 alpha1 L1 ->
     PA_cyclic_pre (substitution A n (succ (var n))) d2 alpha2 L2 ->
-    PA_cyclic_pre (lor C (univ n A)) (max d1 d2) (ord_succ (ord_add (ord_mult alpha2 (wcon (wcon Zero 0 Zero) 0 Zero)) alpha1)) (((univ n A) :: remove form_eq_dec A L2) ++ L1)
+    PA_cyclic_pre (lor C (univ n A)) (max d1 d2) (ord_succ (ord_add alpha1 (ord_mult alpha2 (wcon (wcon Zero 0 Zero) 0 Zero)))) (((univ n A) :: remove form_eq_dec A L2) ++ L1)
 
 | cut1 : forall (C A : formula) {d1 d2 : nat} {alpha1 alpha2 : ord} {L1 L2 : list formula},
     PA_cyclic_pre (lor C A) d1 alpha1 L1 ->
@@ -226,7 +226,7 @@ try apply TA.
 
 1 : apply n.
 
-all : refine ((nf_add _ _ (nf_mult _ _ IHT2 _) IHT1));
+all : refine ((nf_add _ _ IHT1 (nf_mult _ _ IHT2 _)));
       repeat apply single_nf;
       apply zero_nf.
 Qed.
